tests/coq/hashmap/Examples.v
@@ -1,0 +1,103 @@
+
+Require Import Primitives.
+Import Primitives.
+Require Import Coq.ZArith.ZArith.
+Require Import Coq.Lists.List.
+Local Open Scope Primitives_scope.
+Require Import Hashmap_Types.
+Import Hashmap_Types.
+Require Import Hashmap_Funs.
+Import Hashmap_Funs.
+Require Import Lia.
+Require Import Coq.Unicode.Utf8.
+Require Import Coq.Program.Basics.
+Require Import Coq.Program.Equality.
+Require Import Coq.Logic.ProofIrrelevance.
+Require Import Coq.Bool.Bool.
+
+(*    +----------------+
+      | Hint databases |
+      +----------------+
+*)
+Module Example_Hints.
+
+(* Let's make a lemma on a new nat type addition: *)
+
+Inductive int :=
+  | _0 : int
+  | _S : int -> int.
+
+Fixpoint add (a b: int) : int :=
+  match a with
+  | _0    => b
+  | _S a' => _S (add a' b)
+  end.
+
+Lemma add_zero_r a : add a _0 = a.
+Proof.
+induction a.
+- reflexivity.
+- simpl. now rewrite IHa.
+Qed.
+
+(* It cannot be proven with the 'auto' tactic alone. *)
+
+Lemma add_zero_r0 a : add a _0 = a.
+auto. Admitted.
+
+(* However, we can register lemmas in databases that can be used by 'auto' with "Hint Resolve". Here, we implicitly create a new database "ints". *)
+
+Global Hint Resolve add_zero_r: ints.
+
+(* 'auto' can call lemmas of a given database. *)
+
+Example e1 a : add a _0 = a.
+auto with ints. Qed.
+
+Example e2 a : a = add a _0.
+auto with ints. Qed.
+
+(* However, it's stuck if the same lemma need to be applied multiple times. *)
+
+Example e3 a : add (add a _0) _0 = a.
+auto with ints. Admitted.
+
+(* To do that, we can register lemmas in a rewriting database with "Hint Rewrite". Note that this "ints" is not the same database as the one above. *)
+
+Global Hint Rewrite ->add_zero_r0: ints.
+
+Example e4 a : add a _0 = a.
+now autorewrite with ints. Qed.
+
+Example e5 a : a = add a _0.
+now autorewrite with ints. Qed.
+
+Example e6 a : add (add a _0) _0 = a.
+now autorewrite with ints. Qed.
+
+(* By default, 'auto' applies hints from the core database. *)
+
+Global Hint Resolve add_zero_r: core.
+
+Example e7 a : add a _0 = a.
+auto. Qed.
+
+End Example_Hints.
+
+(*    +------------------+
+      | Constants issues |
+      +------------------+
+
+We cannot straightforwardly state properties about any constant, seemingly because the reduction is stuck under ∀.
+
+However, may not want lemmas like that.
+
+Example e1 ty (z: Z) : z = to_Z ((mk_scalar ty z)%return).
+
+Example e2 (n: usize) :
+  ∃z, (n = z%usize).
+*)
+
+(* Search *)
+
+Search (S _ >= _).
